io/TODO.md
@@ -6,7 +6,7 @@ X. `IIO.fst` - assumption in the definition of `dm_giio_bind`.
 
 X. `IIO.fst` - admit in definition of `dm_giio_subcomp`
 
-4. `Hist.fst` - admitted lemma `lemma_hist_bind_associativity` (used in `DMFree.fst`)
+X. `Hist.fst` - admitted lemma `lemma_hist_bind_associativity` (used in `DMFree.fst`)
 
 5. `CommonUtils.fst` - a few admits (not sure if used anymore)
 
